theories/interop/weakestpre.v
@@ -67,8 +67,7 @@ Definition C_state_interp (ζ : lstore) (χ : lloc_map) (θ : addr_map) (roots :
 Definition per_location_invariant_ML (ζ ζvirt : lstore)
      (γ : lloc) (ℓ : loc) : iProp Σ :=
   ∃ (vs : list val) tg lvs, 
-    ( ℓ ↦M/ ∗ ⌜ζ !! γ = Some (Bvblock (Mut, (tg, lvs)))⌝)
-  ∨ (⌜ζ !! γ = None⌝ ∗ γ ↦mut (tg, lvs) ∗ γ ~ℓ~ ℓ)
+    (⌜ζ !! γ = None⌝ ∗ γ ↦mut (tg, lvs) ∗ γ ~ℓ~ ℓ)
   ∨ (⌜ζ !! γ = None⌝ ∗ ⌜ζvirt !! γ = None⌝ ∗ γ ~ℓ~ ℓ).
 
 Definition SI_block_level_ML (ζ : lstore) (χ : lloc_map) : iProp Σ :=
@@ -179,10 +178,9 @@ Proof.
   iIntros (Hnℓ) "Hbig".
   iApply (big_sepM_wand with "Hbig").
   iApply (big_sepM_intro).
-  iIntros "!>" (γ2 ℓ Hne) "(%vs'&%tg&%lvs&[(HNσ&%H1)|[(%H1&Hζ&Hsim)|(%H1&%H2&Hsim)]])"; iExists vs', tg, lvs.
-  - iLeft; by iFrame.
-  - iRight. iLeft. iFrame. done.
-  - iRight. iRight. iFrame. iSplit; first done.
+  iIntros "!>" (γ2 ℓ Hne) "(%vs'&%tg&%lvs&[(%H1&Hζ&Hsim)|(%H1&%H2&Hsim)])"; iExists vs', tg, lvs.
+  - iLeft. iFrame. done.
+  - iRight. iFrame. iSplit; first done.
     iPureIntro. rewrite lookup_insert_ne; first done.
     intros ->. congruence.
 Qed.
@@ -195,10 +193,9 @@ Proof.
   iIntros (Hnℓ) "Hbig".
   iApply (big_sepM_wand with "Hbig").
   iApply (big_sepM_intro).
-  iIntros "!>" (γ2 ℓ Hne) "(%vs'&%tg&%lvs&[(HNσ&%H1)|[(%H1&Hζ&Hsim)|(%H1&%H2&Hsim)]])"; iExists vs', tg, lvs.
-  - iLeft; by iFrame.
-  - iRight. iLeft. iFrame. done.
-  - iRight. iRight. iFrame. iSplit; first done.
+  iIntros "!>" (γ2 ℓ Hne) "(%vs'&%tg&%lvs&[(%H1&Hζ&Hsim)|(%H1&%H2&Hsim)])"; iExists vs', tg, lvs.
+  - iLeft. iFrame. done.
+  - iRight. iFrame. iSplit; first done.
     iPureIntro. rewrite lookup_delete_ne; first done.
     intros ->. congruence.
 Qed.
@@ -218,11 +215,10 @@ Proof.
   iIntros (Hnℓ) "Hbig".
   iApply (big_sepM_wand with "Hbig").
   iApply (big_sepM_intro).
-  iIntros "!>" (γ2 ℓ Hne) "(%vs'&%tg&%lvs&[(HNσ&%H1)|[(%H1&Hζ&Hsim)|(%H1&%H2&Hsim)]])"; iExists vs', tg, lvs.
-  - iLeft; iFrame; iPureIntro; try done. rewrite lookup_delete_ne; try done. intros ->; simplify_eq.
-  - iRight. iLeft. iFrame. iPureIntro.
+  iIntros "!>" (γ2 ℓ Hne) "(%vs'&%tg&%lvs&[(%H1&Hζ&Hsim)|(%H1&%H2&Hsim)])"; iExists vs', tg, lvs.
+  - iLeft. iFrame. iPureIntro.
     by apply delete_lookup_None.
-  - iRight. iRight. iFrame. iSplit; last done. iPureIntro.
+  - iRight. iFrame. iSplit; last done. iPureIntro.
     by apply delete_lookup_None.
 Qed.
 
