theories/interop/wp_utils.v
@@ -192,18 +192,5 @@ Qed.
 
 End RootsRepr.
 
-Lemma interp_ML_discarded_locs_pub χpub (σ:store) :
-    gen_heap_interp σ
- -∗ ([∗ map] ℓ ∈ χpub, ℓ ↦M/)
- -∗ ⌜map_Forall (λ (_ : nat) (ℓ : loc), σ !! ℓ = Some None) χpub⌝.
-Proof.
-  induction χpub as [|k l χpub Hin IH] using map_ind; iIntros "HH HK".
-  - iPureIntro. apply map_Forall_empty.
-  - iPoseProof (big_sepM_insert) as "[HL _]". 1: apply Hin.
-    iPoseProof ("HL" with "HK") as "[H1 H2]".
-    iPoseProof (IH with "HH H2") as "%HIH".
-    iPoseProof (gen_heap_valid with "HH H1") as "%Hv".
-    iPureIntro. apply map_Forall_insert. 1: done. split; done.
-Qed.
 
 End Utils.
